proof/crefine/RISCV64/PSpace_C.thy
@@ -36,14 +36,54 @@ lemma setObject_obj_at_pre:
   apply clarsimp
   done
 
+lemma setObject_ccorres_helper_variable_size:
+  fixes ko :: "'a :: pspace_storable"
+  assumes valid: "\<And>\<sigma> (ko' :: 'a).
+        \<Gamma> \<turnstile> {s. (\<sigma>, s) \<in> rf_sr \<and> P \<sigma> \<and> s \<in> P' \<and> ko_at' ko' p \<sigma>}
+              c {s. (\<sigma>\<lparr>ksPSpace := (ksPSpace \<sigma>)(p \<mapsto> injectKO ko)\<rparr>, s) \<in> rf_sr}"
+  shows "\<lbrakk> \<And>ko :: 'a. updateObject ko = updateObject_default ko;
+           (1 :: machine_word) < 2 ^ objBits ko \<rbrakk>
+    \<Longrightarrow> ccorres dc xfdc (P and obj_at' (\<lambda>obj. objBits ko = objBits obj) p) P' hs (setObject p ko) c"
+  apply (rule ccorres_guard_imp2)
+   apply (subst setObject_obj_at_pre)
+     apply simp+
+   apply (rule ccorres_symb_exec_l[where Q'="\<lambda>_. P'"])
+      defer
+      apply (rule stateAssert_inv)
+     apply (rule stateAssert_sp[where P="P and obj_at' (\<lambda>obj. objBits ko = objBits obj) p"])
+    apply (rule empty_fail_stateAssert)
+   apply fastforce
+  apply (rule ccorres_from_vcg)
+  apply (rule allI)
+  apply (rule hoare_complete)
+  apply (clarsimp simp: HoarePartialDef.valid_def)
+  apply (simp add: typ_at_to_obj_at' koTypeOf_injectKO)
+  apply (drule obj_at_ko_at', clarsimp)
+  apply (drule obj_at_ko_at', clarsimp)
+  apply (cut_tac \<sigma>1=\<sigma> and ko'1=koaa in valid)
+  apply (drule hoare_sound,
+         clarsimp simp: cvalid_def HoarePartialDef.valid_def)
+  apply (elim allE, drule(1) mp)
+  apply (drule mp, simp)
+  apply clarsimp
+  apply (rule imageI[OF CollectI])
+  apply (frule_tac v=ko in setObject_eq_variable_size)
+     apply fastforce
+    apply fastforce
+   apply (fastforce simp: obj_at'_def)
+  apply fastforce
+  done
+
+(* FIXME RT: prove via setObject_ccorres_helper_variable_size, or remove this lemma
+             in favour of setObject_ccorres_helper_variable_size *)
 lemma setObject_ccorres_helper:
   fixes ko :: "'a :: pspace_storable"
   assumes valid: "\<And>\<sigma> (ko' :: 'a).
         \<Gamma> \<turnstile> {s. (\<sigma>, s) \<in> rf_sr \<and> P \<sigma> \<and> s \<in> P' \<and> ko_at' ko' p \<sigma>}
               c {s. (\<sigma>\<lparr>ksPSpace := (ksPSpace \<sigma>)(p \<mapsto> injectKO ko)\<rparr>, s) \<in> rf_sr}"
   shows "\<lbrakk> \<And>ko :: 'a. updateObject ko = updateObject_default ko;
-           \<And>ko :: 'a. (1 :: machine_word) < 2 ^ objBits ko ;
-           \<And>(v :: 'a) (v' :: 'a). objBits v = objBits v'\<rbrakk>
+           \<And>ko :: 'a. (1 :: machine_word) < 2 ^ objBits ko;
+           \<And>(v :: 'a) (v' :: 'a). objBits v = objBits v' \<rbrakk>
     \<Longrightarrow> ccorres dc xfdc P P' hs (setObject p ko) c"
   apply (rule ccorres_guard_imp2)
    apply (subst setObject_obj_at_pre)
@@ -111,6 +151,50 @@ lemma storePTE_Basic_ccorres:
   apply (rule ccorres_guard_imp2)
    apply (erule storePTE_Basic_ccorres')
   apply simp
+  done
+
+lemma ccorres_pre_getObject_sc:
+  assumes cc: "\<And>rv. ccorres r xf (P rv) (P' rv) hs (f rv) c"
+  shows   "ccorres r xf
+                  (\<lambda>s. (\<forall>sc. ko_at' sc p s \<longrightarrow> P sc s))
+                  {s. \<forall> sc sc'. cslift s (Ptr p) = Some sc' \<and> csched_context_relation sc sc'
+                           \<longrightarrow> s \<in> P' sc}
+                          hs (getSchedContext p >>= (\<lambda>rv :: sched_context. f rv)) c"
+  apply (rule ccorres_guard_imp2)
+   apply (rule ccorres_symb_exec_l)
+      apply (rule ccorres_guard_imp2)
+       apply (rule cc)
+      apply (rule conjI)
+       apply (rule_tac Q="ko_at' rv p s" in conjunct1)
+       apply assumption
+      apply assumption
+     apply (wpsimp wp: set_sc'.getObject_wp empty_fail_getObject simp: getSchedContext_def)+
+  apply (erule cmap_relationE1[OF cmap_relation_sched_context],
+         erule ko_at_projectKO_opt)
+  apply simp
+  done
+
+lemma updateSchedContext_eq:
+  "\<lbrakk>ko_at' sc scPtr s; objBits sc < word_bits; \<And>sc. scSize (f sc) = scSize sc\<rbrakk>
+   \<Longrightarrow> ((), s\<lparr> ksPSpace := (ksPSpace s)(scPtr \<mapsto> injectKO (f sc))\<rparr>)
+       \<in> fst (updateSchedContext scPtr f s)"
+  unfolding updateSchedContext_def
+  apply (clarsimp simp add: in_monad)
+  apply (rule exI)
+  apply (rule exI)
+  apply (rule conjI)
+   apply (clarsimp simp: getSchedContext_def)
+   apply (rule getObject_eq)
+     apply simp
+   apply assumption
+  apply (frule_tac v="f sc" in setObject_eq_variable_size)
+     apply simp
+    apply (simp add: objBits_simps')
+    using scBits_pos_power2 apply fastforce
+   apply (simp add: obj_at'_def)
+   apply (rule_tac x=sc in exI)
+   apply (simp add: objBits_simps)
+  apply (clarsimp simp: setSchedContext_def)
   done
 
 end
